lakefile.lean
@@ -5,6 +5,6 @@ package MLIRSemantics {
   binRoot := `MLIRSemantics
   dependencies := #[{
     name := "MLIR",
-    src := Source.git "https://github.com/lephe/lean-mlir.git" "5d29c1c1494e189cc1e519875534f52749fc1f5a",
+    src := Source.git "https://github.com/lephe/lean-mlir.git" "feb5e250ef4da51408ebdc75b6e7cbd24c96b73e",
   }]
 }
